@prefix ceterms: <http://purl.org/ctdl/terms/> .
@prefix dct: <http://purl.org/dc/terms/> .
@prefix lmt: <https://opensource.ieee.org/lmt/terms/> .
@prefix lrmi: <http://purl.org/dcx/lrmi-terms/> .
@prefix owl: <http://www.w3.org/2002/07/owl#> .
@prefix rdf: <http://www.w3.org/1999/02/22-rdf-syntax-ns#> .
@prefix rdfs: <http://www.w3.org/2000/01/rdf-schema#> .
@prefix scd: <https://opensource.ieee.org/scd/terms/> .
@prefix sdo: <http://schema.org/> .
@prefix skos: <http://www.w3.org/2004/02/skos/core#> .
@prefix xsd: <http://www.w3.org/2001/XMLSchema#> .

<https://opensource.ieee.org/lmt/terms/> a rdfs:Class ;
    dct:description "An RDF vocabulary for describing the RDF classes, properties defined in the LMT namespace."@en ;
    dct:title "Learning Metadata terms"@en  .
    
#------------
# CLASSES
#------------

lmt:LearningEvent a rdfs:Class ;
    rdfs:label "Learning Event"@en ;
    rdfs:comment "An event based on a LearningResource."@en ;
    dct:description "An ephemeral resource with unique combinations of time, space (place), agency and other event-specific attributes; a fixing (recording) of a LearningEvent in any tangible medium, now known or later developed, results in a new persistent LearningResource."@en-US ;
    rdfs:subClassOf lmt:LearningObject ;
    rdfs:isDefinedBy <https://opensource.ieee.org/lmt/terms/> .
    
lmt:LearningObject a rdfs:Class ;
    rdfs:label "Learning Object"@en ;
    rdfs:comment "An abstract class of which LearningResource and LearningInstantiation are subclasses."@en ;
    rdfs:isDefinedBy <https://opensource.ieee.org/lmt/terms/> .
    
lmt:LearningResource a rdfs:Class ;
    rdfs:label "Learning Resource"@en ;
    rdfs:comment "A persistent resource that has one or more physical or digital representations, and that explicitly involves, specifies, or entails a learning activity or learning experience."@en ;
    rdfs:isDefinedBy <https://opensource.ieee.org/lmt/terms/> .
    
#------------
# PROPERTIES
#------------
    
lmt:hasEvent a rdf:Property ;
    rdfs:label "has event"@en ;
    rdfs:comment "A related event based on this LearningResource."@en ;
    sdo:domainIncludes <https://opensource.ieee.org/lmt/terms/LearningResource> ;
    sdo:rangeIncludes <https://opensource.ieee.org/lmt/terms/LearningEvent> ; 
    rdfs:isDefinedBy <https://opensource.ieee.org/lmt/terms/> .
    
lmt:hasRepresentation a rdf:Property ;
    rdfs:label "has representation"@en ;
    rdfs:comment "A related LearningResource representing the same work and expression in a different tangible medium (format)."@en ;
    dct:description "For a related resource that alters the work and expression, use either the hasVersion or isBasedOn property depending on the circumstances."@en-US ;
    sdo:domainIncludes <https://opensource.ieee.org/lmt/terms/LearningResource> ;
    sdo:rangeIncludes <https://opensource.ieee.org/lmt/terms/LearningResource> ; 
    rdfs:isDefinedBy <https://opensource.ieee.org/lmt/terms/> .
    
lmt:isEventOf a rdf:Property ;
    rdfs:label "is event of"@en ;
    rdfs:comment "The LearningResource on which this LearningEvent is based."@en ;
    sdo:domainIncludes <https://opensource.ieee.org/lmt/terms/LearningResource> ;
    sdo:rangeIncludes <https://opensource.ieee.org/lmt/terms/LearningEvent> ; 
    rdfs:isDefinedBy <https://opensource.ieee.org/lmt/terms/> .