@prefix asn: <http://purl.org/ASN/schema/core/> .
@prefix ceasn: <https://purl.org/ctdlasn/terms/> .
@prefix ceterms: <https://purl.org/ctdl/terms/> .
@prefix dct: <http://purl.org/dc/terms/> .
@prefix frbr: <http://iflastandards.info/ns/fr/frbr/frbrer/> .
@prefix lmt: <https://opensource.ieee.org/lmt/terms/> .
@prefix lrmi: <http://purl.org/dcx/lrmi-terms/> .
@prefix owl: <http://www.w3.org/2002/07/owl#> .
@prefix rdf: <http://www.w3.org/1999/02/22-rdf-syntax-ns#> .
@prefix rdfs: <http://www.w3.org/2000/01/rdf-schema#> .
@prefix scd: <https://opensource.ieee.org/scd/terms/> .
@prefix sdo: <http://schema.org/> .
@prefix skos: <http://www.w3.org/2004/02/skos/core#> .
@prefix xsd: <http://www.w3.org/2001/XMLSchema#> .

<https://opensource.ieee.org/lmt/terms/> a rdfs:Class ;
    dct:description "An TEMPORARY RDF profile vocabulary for describing the RDF classes, properties, and concepts of a learning object that have been: (1) defined in an LMT namespace; and (2) reused from other namespaces."@en ;
    dct:title "Learning Metadata terms"@en  .
    
#------------
# CLASSES
#------------

lmt:LearningEvent a rdfs:Class ;
    rdfs:label "Learning Event"@en ;
    rdfs:comment "A temporal opportunity or manifestation for learning that is contextualized around resourcing constraints, such as time, space, and cost."@en ;
    skos:note "An ephemeral resource with unique combinations of time, space (place), agency and other event-specific attributes; a fixing (recording) of a LearningEvent in any tangible medium, now known or later developed, results in a new persistent LearningResource."@en-US ;
    rdfs:subClassOf lmt:LearningObject ;
    rdfs:isDefinedBy <https://opensource.ieee.org/lmt/terms/> .
    
lmt:LearningObject a rdfs:Class ;
    rdfs:label "Learning Object"@en ;
    rdfs:comment "The abstract class of all metadata descriptions of both ephemeral learning events and persistent resources that explicitly involve, specify, or entail a learning activity or learning experience."@en ;
    skos:note "A superclass of which LearningResource and LearningEvent used in metadata descriptions are subclasses. The LearningObject class should not be used directly in metadata descriptions where the LearningEvent and LearningResource subclasses are adequate."@en ;
    rdfs:isDefinedBy <https://opensource.ieee.org/lmt/terms/> .
    
lrmi:LearningResource a rdfs:Class ;
    rdfs:label "Learning Resource"@en ;
    rdfs:comment "A persistent resource that has one or more physical or digital representations, and that explicitly involves, specifies or entails a learning activity or learning experience."@en ;
    skos:scopeNote "LearningResource is expected to be used as an addition to a primary type such as http://purl.org/ontology/bibo/Book, https://schema.org/Video, http://purl.org/dc/terms/PhysicalResource etc."@en ;
    skos:note "LMT Annotation: The LearningResource is intended to function as a digital resource that is usable and shareable, and can be rich in context."@en ;
    rdfs:isDefinedBy <http://purl.org/dcx/lrmi-terms/> .
    
#------------
# PROPERTIES
#------------

lrmi:assesses a rdf:Property ;
    rdfs:label "assesses"@en ;
    rdfs:comment "The item being described is intended to assess the competency or learning outcome defined by the referenced term."@en ;
    sdo:domainIncludes  
        <https://opensource.ieee.org/lmt/terms/LearningResource> ,
        <https://opensource.ieee.org/lmt/terms/LearningEvent> ;
    sdo:rangeIncludes 
        <https://opensource.ieee.org/scd/terms/CompetencyDefinition> ,
        <https://purl.org/ctdlasn/terms/Competency> ,
        <http://purl.org/ASN/schema/core/Statement> ;
    rdfs:isDefinedBy <http://purl.org/dcx/lrmi-terms/> ;
    
dct:audience a rdf:Property ;
    rdfs:label "audience"@en ;
    rdfs:comment "Class of agents for whom the resource is intended or useful."@en ;
    skos:note "Recommended practice is to use this property with non-literal values from a vocabulary of audience types."@en ;
    sdo:domainIncludes  
        <https://opensource.ieee.org/lmt/terms/LearningResource> ,
        <https://opensource.ieee.org/lmt/terms/LearningEvent> ;
    sdo:rangeIncludes <http://purl.org/dc/terms/AgentClass> ;
    rdfs:isDefinedBy <http://purl.org/dc/terms/> .
    
dct:description a rdf:Property ;
    rdfs:label "description"@en ;
    rdfs:comment "An account of the resource."@en ;
    skos:sopeNote "Description may include but is not limited to: an abstract, a table of contents, a graphical representation, or a free-text account of the resource."@en ;
    sdo:domainIncludes  
        <https://opensource.ieee.org/lmt/terms/LearningResource> ,
        <https://opensource.ieee.org/lmt/terms/LearningEvent> ;
    sdo:rangeIncludes <http://www.w3.org/1999/02/22-rdf-syntax-ns#langString> ;
    rdfs:isDefinedBy <http://purl.org/dc/terms/> .
    
lrmi:educationLevel a rdf:Property ;
    rdfs:label "education level"@en ;
    rdfs:comment "The level of a resource in terms of progression through an educational or training context."@en ;
    skos:example "Examples of educational levels include 'beginner', 'intermediate' or 'advanced', and formal sets of level indicators."@en ;
    sdo:domainIncludes  
        <https://opensource.ieee.org/lmt/terms/LearningResource> ,
        <https://opensource.ieee.org/lmt/terms/LearningEvent> ;
    sdo:rangeIncludes <http://www.w3.org/2004/02/skos/core#Concept> ;
    rdfs:isDefinedBy <http://purl.org/dcx/lrmi-terms/> .
    
dct:format a rdf:Property ;
    rdfs:label "format"@en ;
    rdfs:comment "The file format, physical medium, or dimensions of the resource."@en ;
    skos:scopeNote "Recommended practice is to use a controlled vocabulary where available. For example, for file formats one could use the list of Internet Media Types [MIME]. Examples of dimensions include size and duration.@en ;
    skos:note "LMT Annotation: The format property is constrained to just the InternetMediaType [MIME]"@en ; 
    sdo:domainIncludes <https://opensource.ieee.org/lmt/terms/LearningResource> ,
    sdo:rangeIncludes <https://www.iana.org/assignments/media-types/media-types.xhtml> ; 
    rdfs:isDefinedBy <http://purl.org/dc/terms/> .
    
frbr:hasAdaption a rdf:Property ;
    rdfs:label "has adaption"@en ;
    rdfs:comment "Relates a prior work to another work that represents a modification of the content of the prior work for a purpose, use, or medium other than that for which it was originally intended. "@en ;
    skos:note "LMT Annotation: The modification of the content of the prior work must be sufficient in degree to warrant the adaptated work being considered as a new work autonomous with respect to the work being adapted. If the change does not alter the original intention, use dct:hasVersion."@en ;
    sdo:domainIncludes <https://opensource.ieee.org/lmt/terms/LearningResource> ;
    sdo:rangeIncludes <https://opensource.ieee.org/lmt/terms/LearningResource> ;    
    rdfs:isDefinedBy <http://iflastandards.info/ns/fr/frbr/frbrer/> .

lmt:hasEvent a rdf:Property ;
    rdfs:label "has event"@en ;
    rdfs:comment "A related event based on this LearningResource."@en ;
    sdo:domainIncludes <https://opensource.ieee.org/lmt/terms/LearningResource> ;
    sdo:rangeIncludes <https://opensource.ieee.org/lmt/terms/LearningEvent> ; 
    rdfs:isDefinedBy <https://opensource.ieee.org/lmt/terms/> .
    
lmt:hasFormat a rdf:Property ;
    rdfs:label "has format"@en ;
    rdfs:comment "A related resource that is substantially the same as the pre-existing described resource, but in another format."@en ;
    skos:scopeNote "This property is intended to be used with non-literal values. This property is an inverse property of Is Format Of."@en ;
    sdo:domainIncludes <https://opensource.ieee.org/lmt/terms/LearningResource> ;
    sdo:rangeIncludes <https://opensource.ieee.org/lmt/terms/LearningR> ; 
    rdfs:isDefinedBy <https://opensource.ieee.org/lmt/terms/> .
    
dct:hasPart a rdf:Property ;
    rdfs:label "has part"@en ;
    rdfs:comment "A related resource that is included either physically or logically in the described resource."@en ;
    sdo:domainIncludes  <https://opensource.ieee.org/lmt/terms/LearningResource> ;
    sdo:rangeIncludes 
        <https://opensource.ieee.org/lmt/terms/LearningResource> ,
        <https://opensource.ieee.org/lmt/terms/LearningEvent> ;
    rdfs:isDefinedBy <http://purl.org/dc/terms/> .
    
dct:hasVersion a rdf:Property ;
    rdfs:label "has version"@en ;
    rdfs:comment "A related resource that is a version, edition, or adaptation of the described resource."@en ;
    skos:scopeNote "Changes in version imply substantive changes in content rather than differences in format. This property is intended to be used with non-literal values. This property is an inverse property of Is Version Of."@en ;
    skos:note "LMT Annotation: A linked revision of this object, pointing forward to the revised object. It is expected that revisions happen internal to an organization.  Note that what constitutes an \"adaptation\" is broad and both \"hasRepresentation\" and \"isBasedOn\" should be consulted before determining if this property is appropriate for the type of modification."@en ;
    sdo:domainIncludes <https://opensource.ieee.org/lmt/terms/LearningResource> ;
    sdo:rangeIncludes <https://opensource.ieee.org/lmt/terms/Learningresource> ; 
    rdfs:isDefinedBy <http://purl.org/dc/terms/> .
    
dct:instructionalMethod a rdf:Property ;
    rdfs:label "instructional method"@en ;
    rdfs:comment "A process, used to engender knowledge, attitudes and skills, that the described resource is designed to support."@en ;
    dct:description "Instructional Method typically includes ways of presenting instructional materials or conducting instructional activities, patterns of learner-to-learner and learner-to-instructor interactions, and mechanisms by which group and individual levels of learning are measured. Instructional methods include all aspects of the instruction and learning processes from planning and implementation through evaluation and feedback."@en-US ;
    sdo:domainIncludes  
        <https://opensource.ieee.org/lmt/terms/LearningResource> ,
        <https://opensource.ieee.org/lmt/terms/LearningEvent> ;
    sdo:rangeIncludes <http://www.w3.org/2004/02/skos/core#Concept>  ;
    rdfs:isDefinedBy <http://purl.org/dc/terms/> .
    
sdo:instructor a rdf:Property ;
    rdfs:label "instructor"@en ;
    rdfs:comment "A person assigned to instruct or provide instructional assistance for the CourseInstance."@en ;
    sdo:domainIncludes <https://opensource.ieee.org/lmt/terms/LearningEvent> ;
    sdo:rangeIncludes <http://schema.org/Person> ; 
    rdfs:isDefinedBy <http://schema.org/> .
    
lmt:isEventOf a rdf:Property ;
    rdfs:label "is event of"@en ;
    rdfs:comment "The LearningResource on which this LearningEvent is based."@en ;
    sdo:domainIncludes <https://opensource.ieee.org/lmt/terms/LearningResource> ;
    sdo:rangeIncludes <https://opensource.ieee.org/lmt/terms/LearningEvent> ; 
    rdfs:isDefinedBy <https://opensource.ieee.org/lmt/terms/> .
    
dct:isPartOf a rdf:Property ;
    rdfs:label "is part of"@en ;
    rdfs:comment "A related resource in which the described resource is physically or logically included."@en ;
    sdo:domainIncludes <https://opensource.ieee.org/lmt/terms/LearningResource> ;
    sdo:rangeIncludes <https://opensource.ieee.org/lmt/terms/LearningResource> ;
    rdfs:isDefinedBy <http://purl.org/dc/terms/> .
    
dct:isVersionOf a rdf:Property ;
    rdfs:label "is version of"@en ;
    rdfs:comment "A related resource of which the described resource is a version, edition, or adaptation."@en ;
    sdo:domainIncludes <https://opensource.ieee.org/lmt/terms/LearningResource> ;
    sdo:rangeIncludes <https://opensource.ieee.org/lmt/terms/LearningResource> ;
    rdfs:isDefinedBy <http://purl.org/dc/terms/> .
    
sdo:keywords a rdf:Property ;
    rdfs:label "keywords"@en ;
    rdfs:comment "Keywords or tags used to describe some item."@en ;
    dct:description "Multiple textual entries in a keywords list are typically delimited by commas, or by repeating the property."@en-US ;
    sdo:domainIncludes <https://opensource.ieee.org/lmt/terms/LearningResource> ;
    sdo:rangeIncludes <https://opensource.ieee.org/lmt/terms/LearningResource> ; 
    rdfs:isDefinedBy <http://schema.org/> .
    
dct:language a rdf:Property ;
    rdfs:label "language"@en ;
    rdfs:comment "A language of the resource."@en ;
    dct:description "Recommended practice is to use either a non-literal value representing a language from a controlled vocabulary such as ISO 639-2 or ISO 639-3, or a literal value consisting of an IETF Best Current Practice 47 [IETF-BCP47] language tag."@en-US ;
    sdo:domainIncludes  
        <https://opensource.ieee.org/lmt/terms/LearningResource> ,
        <https://opensource.ieee.org/lmt/terms/LearningEvent> ;
    sdo:rangeIncludes 
        <http://www.w3.org/2004/02/skos/core#Concept> ,
        <http://www.w3.org/2000/01/rdf-schema#Literal> ;
    rdfs:isDefinedBy <http://purl.org/dc/terms/> .
    
sdo:offeredBy a rdf:Property ;
    rdfs:label "offered by"@en ;
    rdfs:comment "A pointer to the organization or person making the offer."@en ;
    sdo:domainIncludes 
        <https://opensource.ieee.org/lmt/terms/LearningResource> ,
        <https://opensource.ieee.org/lmt/terms/LearningEvent> ;
    sdo:rangeIncludes 
        <http://schema.org/CollegeOrUniversity> ,
        <http://schema.org/Organization> ; 
    rdfs:isDefinedBy <http://schema.org/> .
    
ceterms:ownedBy a rdf:Property ;
    rdfs:label "owned by"@en ;
    rdfs:comment "Organization or person with an enforceable claim or legal title to the resource."@en ;
    sdo:domainIncludes 
        <https://opensource.ieee.org/lmt/terms/LearningResource> ,
        <https://opensource.ieee.org/lmt/terms/LearningEvent> ;
    sdo:rangeIncludes 
        <http://schema.org/CollegeOrUniversity> ,
        <http://schema.org/Organization> ; 
    rdfs:isDefinedBy <http://schema.org/> .
    
dct:spatial a rdf:Property ;
    rdfs:label "spatial"@en ;
    rdfs:comment "Spatial characteristics of the resource."@en ;
    dct:description "A spatial/geographic region or a named place."@en-US ;
    sdo:domainIncludes  
        <https://opensource.ieee.org/lmt/terms/LearningResource> ,
        <https://opensource.ieee.org/lmt/terms/LearningEvent> ;
    sdo:rangeIncludes <http://purl.org/dc/terms/Location> ;
    rdfs:isDefinedBy <http://purl.org/dc/terms/> .

dct:subject a rdf:Property ;
    rdfs:label "subject"@en ;
    rdfs:comment "A topic of the resource."@en ;
    sdo:domainIncludes  
        <https://opensource.ieee.org/lmt/terms/LearningResource> ,
        <https://opensource.ieee.org/lmt/terms/LearningEvent> ;
    sdo:rangeIncludes <http://www.w3.org/2004/02/skos/core#Concept> ;
    rdfs:isDefinedBy <http://purl.org/dc/terms/> .
    
dct:temporal a rdf:Property ;
    rdfs:label "temporal"@en ;
    rdfs:comment "Temporal characteristics of the resource."@en ;
    dct:description "Temporal characteristics may denote either aspects of the subject matter of the resource (e.g., a named historical era) or aspects of the jurisdictional applicability (e.g., where the resource is valid or specifically intended)."@en-US ;
    sdo:domainIncludes  
        <https://opensource.ieee.org/lmt/terms/LearningResource> ,
        <https://opensource.ieee.org/lmt/terms/LearningEvent> ;
    sdo:rangeIncludes <http://www.w3.org/2004/02/skos/core#Concept> ;
    rdfs:isDefinedBy <http://purl.org/dc/terms/> .
    
dct:title a rdf:Property ;
    rdfs:label "title"@en ;
    rdfs:comment "A name given to the resource."@en ;
    dct:description "A basic name for the Learning Object; what one would expect to use to distinguish it from others like it."@en-US ;
    sdo:domainIncludes  
        <https://opensource.ieee.org/lmt/terms/LearningResource> ,
        <https://opensource.ieee.org/lmt/terms/LearningEvent> ;
    sdo:rangeIncludes <http://www.w3.org/2000/01/rdf-schema#langString> ;
    rdfs:isDefinedBy <http://purl.org/dc/terms/> .   